\documentclass{article}
\usepackage{amsmath}
\usepackage{amsfonts}
\usepackage{fullpage}
\usepackage{verbatim}

\renewcommand{\epsilon}{\varepsilon}

\title{Homework 2}
\author{Geoff Hotchkiss}

\begin{document}
\maketitle

\noindent {\bf Theorem 1:} Suppose that $f(n) = O(g(n))$. Then $g(n) = \Omega(f(n))$. \\
{\bf Proof:} We have that $f(n) = O(g(n))$. Then there exists constants $n_0 \geq 0$ and $c > 0$ such that $f(n) \leq c \cdot g(n)$ for all $n \geq n_0$.
Since $c > 0$, it follows that $\frac{1}{c} > 0$ and $\frac{1}{c} \cdot f(n) \leq g(n)$. Let $\epsilon = \frac{1}{c}$ and let $n_0' = n_0$. Then there exists constants
$\epsilon > 0$ and $n_0' \geq 0$ such that for all $n \geq  n_0'$, $g(n) \geq \epsilon \cdot f(n)$ which is the definition of $g(n) = \Omega(f(n))$.

\begin{enumerate}
	\item $\ln(n!), (\ln n)!$ \\
				Since $(\ln n)! > \ln(n!)$ for all $n > 1500$, we have that $\ln(n!) = O((\ln n)!)$. \\ \\
				I can't figure out how to show that $(\ln n)! \neq O(\ln(n!))$.
	
	\item $3n^2 + 17n, \frac{1}{3}n^3$ \\
				$3^2 + 17n = O(\frac{1}{3}n^3)$ \\
				{\bf Proof:} 
				\begin{align*}
					3n^2 + 17n & \leq 3n^3 + 17n^3 \quad \text{for $n \geq 1$} \\
										 & = 20n^3 \\
										 & = 60 \cdot \frac{1}{3}n^3.
				\end{align*}
				Thus, $n_0 = 1$ and $c = 60$. \\ \\
				We need to show that $\frac{1}{3}n^3 \neq O(3n^2 + 17n)$. Thus we want to show that for all $c > 0$ and $n_0 \geq 0$, there exists an $n \geq n_0$
				such that $\frac{1}{3} n^3 > c(3n^2 + 17n)$. Solving this inequality for $n$, we find that $n > \frac{1}{2} \left(9 c+\sqrt{3} \sqrt{68 c+27 c^2}\right)$. Thus, we can let $n = \frac{1}{2} \left(9 c+\sqrt{3} \sqrt{68 c+27 c^2}\right) + n_0 + 1 > n_0$ and we are done.
				
	\item $\displaystyle n^{\frac{1}{\ln n}}, n^2$ \\ \\
				$\displaystyle n^{\frac{1}{\ln n}} = O(n^2)$ \\
				{\bf Proof:}
					We have that $2 > \frac{1}{\ln{2}} \approx 1.4427$. Thus $2 > \frac{1}{\ln n}$ for $n \geq 2$. Thus $n^2 \geq n^{\frac{1}{\ln n}}$ for 
					$n \geq 2$, with $n_0 \geq 2$ and $c = 1$. \\ \\
				We want to show that $n^2 \neq O(n^{\frac{1}{\ln n}})$. Thus we want to show that for all $c > 0$ and $n_0 \geq 0$, there exists an $n \geq n_0$ 
				such that $n^2 > c \cdot n^{\frac{1}{\ln n}}$. Taking the logarithm of both sides, we obtain $2\ln n > \ln c + 1$. Thus whenever 
				$n > e^{\frac{\ln c + 1}{2}}$ the inequality holds true. Thus, we can let $n = \max(e^{\frac{\ln c + 1}{2}}, n_0) + 1$ and we are done.
					
	\pagebreak
					
	\item $\displaystyle (\ln n)^{\ln n}, n^{\ln \ln n}$. \\
	
				{\bf Claim:} $\displaystyle (\ln n)^{\ln n} = n^{\ln \ln n}$. \\
				{\bf Proof:} Let $\displaystyle f(n) = (\ln n)^{\ln n}$ and $\displaystyle g(n) = n^{\ln \ln n}$. It is sufficient to show that 
				$\ln f(n) = \ln g(n)$. Since $\ln f(n) = (\ln n)(\ln \ln n)$ and $\ln g(n) = (\ln \ln n)(\ln n)$, we are done. \\
				
				{\bf Claim:} $\displaystyle (\ln n)^{\ln n} = O(n^{\ln \ln n})$ and $\displaystyle n^{\ln \ln n} = \Omega((\ln n)^{\ln n})$. \\
				{\bf Proof:} Since we know that the two functions we are concerned with are equal, let $\displaystyle f(n) = (\ln n)^{\ln n}$. Note that 
				$\displaystyle f(n) = n^{\ln \ln n}$ as well. Thus we have that:
					\begin{align*}
						f(n) = (\ln n)^{\ln n} & \leq f(n) \\
																	 & = n^{\ln \ln n} \\
						f(n) = n^{\ln \ln n} & \leq f(n) \\
																 & = (\ln n)^{\ln n},
					\end{align*}
				and we are done. This also shows that they are $\Theta$ of each other since the two original functions are equaliviant.
	
	\item $\displaystyle \ln n , \frac{n}{\ln n}$. \\
	      \begin{comment}
				{\bf Claim:} $\displaystyle \ln n \leq \frac{n}{\ln n}$ for all $n \geq e^4$ and thus $\displaystyle \ln n = O(\frac{n}{\ln n})$. It follows that 
				$\displaystyle \frac{n}{\ln n} = \Omega(\ln n)$. \\
				{\bf Proof:} For all $n \geq e^4$, we have that:
					\begin{align*}
						\ln n & \leq \frac{1}{e^2} n \quad \Rightarrow \\
						e^2 \ln n & \leq n \quad \Rightarrow \\
						e^{2 (\ln \ln n)} & \leq e^{\ln n} \quad \Rightarrow \\
						2 (\ln \ln n) & \leq \ln n \quad \Rightarrow \\
						\ln \ln n & \leq \ln n - \ln \ln n \Rightarrow \\
						\ln n & \leq \frac{n}{\ln n}.
					\end{align*}
				Thus for all $n \geq n_0 = e^4$, we have that $\ln n \leq \frac{n}{\ln n}$. Applying Theorem 1, we have the second part and we are done. Since 
				we have the inequality, they are not $\Theta$ of each other. \\ \\
				\end{comment}
				{\bf Claim:} $\ln n = O(\frac{n}{\ln n})$. \\ 
				{\bf Proof:} We need to show that there exists $c > 0$ and $n_0 \geq 0$ such that $c \cdot \frac{n}{\ln n} \geq \ln n$. Consider 
				$\frac{n}{\ln n} > \ln n$. Since this is true for all $n \geq e$, we can let $n_0 = e$ and $c = 1$.\\ \\ 
				We want to show that $\frac{n}{\ln n} \neq O(\ln n)$. Thus we want to show that for all $c > 0$ and $n_0 \geq 0$, there exists and $n \geq n_0$ 
				such that $\frac{n}{\ln n} > c \ln n$. This simplifies to $\frac{n}{(\ln n)^2} > c$. Since
					\begin{align*}
						\lim_{n \to \infty} \frac{n}{(\ln n)^2} & = \lim_{n \to \infty} \frac{n}{2 \ln n} \\
																										& = \lim_{n \to \infty} \frac{n}{2} = \infty,																					
					\end{align*}
				we can choose an $n' \in \mathbb{Z}^+$ such that $\frac{n'}{(\ln n')^2} > c$. Then let $n = \max(n', n_0) + 1$ and we are done.
				
				
						
\end{enumerate}
\end{document}